infra/NePreSuffix.v
@@ -14,3 +14,38 @@ Proof.
   destruct l;[intros;eapply prefix_nil|
               cbn;intros;eapply prefix_cons;setoid_rewrite nlcons_to_list at 2;eauto].
 Qed.
+
+(** * StrictPrefix **)
+
+Section StrictPre.
+
+  Variable (A : Type).
+
+  Definition StrictPrefix' := 
+    fun (l l' : ne_list A) => exists a : A, Prefix (a :<: l) l'.
+
+  Lemma prefix_strictPrefix:
+    forall (e : A) (x ϕ : ne_list A), Prefix ϕ x -> StrictPrefix' ϕ (e :<: x).
+  Proof.
+    intros e x ϕ Hϕ1.
+    unfold StrictPrefix'. cbn.
+    revert dependent e.
+    induction Hϕ1; intros.
+    - exists e; econstructor.
+    - specialize(IHHϕ1 a). destructH. exists a0. econstructor. auto.
+  Qed.
+
+  Lemma StrictPrefix_well_founded : well_founded (StrictPrefix').
+  Proof.
+    unfold well_founded.
+    intros. 
+    induction a.
+    - econstructor. intros. unfold StrictPrefix' in *. destructH. inversion H;[congruence'|]. inversion H2.
+    - constructor. intros.
+      unfold StrictPrefix' in H.
+      destructH. cbn in *. inversion H;subst.
+      + eapply ne_to_list_inj in H3. subst. auto.
+      + eapply IHa. unfold StrictPrefix'. exists a1. cbn. auto.
+  Qed.
+
+End StrictPre.
