cfg/CFGTac.v
@@ -1,0 +1,33 @@
+Require Export CFGdef.
+
+Open Scope prg.
+
+Ltac to_loop_contains' :=
+  match goal with
+  | [C : redCFG ?edge ?root ?a_edge |- context [loop_contains ?h ?p]]
+    => unfold loop_contains,back_edge,back_edge_b;
+      fold (loop_contains' edge a_edge h p)
+  end.
+
+
+Ltac fold_lp_cont' :=
+  repeat lazymatch goal with
+         | [H : context [exists _ _, (?edge ∖ ?a_edge) _ ?h = true /\ Path ?edge ?q _ _ /\ ?h ∉ tl (rev _) ] |- _]
+           => unfold finType_sub_decPred in H;
+             fold (loop_contains' edge a_edge h q) in H
+         | [H : context [loop_contains' ?edge ?a_edge ?h ?p
+                         /\ ~ loop_contains' ?edge ?a_edge ?h ?q /\ ?edge ?p ?q = true] |- _]
+           => fold (exit_edge' edge a_edge h p q) in H
+         | [ |- context [loop_contains' ?edge ?a_edge ?h ?p
+                        /\ ~ loop_contains' ?edge ?a_edge ?h ?q
+                        /\ ?edge ?p ?q = true]]
+           => fold (exit_edge' edge a_edge h p q)
+         | |- context [exists _ _, (?edge ∖ ?a_edge) _ ?h = true /\ Path ?edge ?q _ _ /\ ?h ∉ tl (rev _)]
+           => unfold finType_sub_decPred;
+             fold (loop_contains' edge a_edge h q)
+         end.
+
+Ltac unfold_edge_op := repeat unfold intersection_edge,restrict_edge',minus_edge,union_edge; conv_bool.
+Ltac unfold_edge_op' H := repeat (unfold intersection_edge,restrict_edge',minus_edge,union_edge in H);
+                          conv_bool.
+
