cfg/CFGgeneral.v
@@ -1,0 +1,26 @@
+Require Export CFGdef CFGTac.
+
+Lemma all_sat_restrict_edge'
+      (L : Type)
+      (f : L -> L -> bool)
+      (p q : L)
+      (π : ne_list L)
+      (Hπ : Path f p q π)
+      (P : decPred L)
+      (Hsat :  forall x : L, x ∈ π -> P x)
+  : Path (restrict_edge' f P) p q π.
+Proof.
+  induction Hπ.
+  - econstructor.
+  - econstructor.
+    + eapply IHHπ. intros; eapply Hsat. cbn. firstorder.
+    + unfold_edge_op; split_conj; eauto; eapply Hsat; cbn; auto.
+      right. eapply path_contains_front;eauto.
+Qed.
+
+Lemma loop_contains'_basic `{redCFG} h p
+  : loop_contains' edge a_edge h p = loop_contains h p.
+Proof.
+  reflexivity.
+Qed.
+
