cfg/CFGloop.v
@@ -1,0 +1,495 @@
+Require Export CFGdef CFGTac.
+
+
+Section cfg.
+  Context `{C : redCFG}.
+
+  Notation "p '-a>b' q" := (a_edge p q) (at level 55).
+  Notation "p '-a>' q" := (p -a>b q = true) (at level 55).
+  Notation "p '-->b' q" := (edge p q) (at level 55).
+  Notation "p '-->' q" := (p -->b q = true) (at level 55, right associativity).
+
+  (** about loops **)
+  
+  Lemma loop_contains_loop_head (qh q : Lab)
+    : loop_contains qh q -> loop_head qh.
+  Proof.
+    intro Q. unfold loop_head, loop_contains in *. destruct Q as [p [_ [Q _]]].
+    eexists; eauto.
+  Qed.
+
+  Lemma loop_contains_self h : loop_head h -> loop_contains h h.
+  Proof.
+    intros Hl. unfold loop_contains.
+    - unfold loop_head in Hl. destruct Hl. 
+      eapply loop_head_dom in H as Hdom.
+      eapply back_edge_incl in H as Hreach. specialize (a_reachability x) as Hreach'.
+      destructH.
+      eapply subgraph_path' in Hreach' as Hreach'';eauto using a_edge_incl.
+      eapply Hdom in Hreach''. eapply path_from_elem in Hreach''; eauto.
+      destructH; eauto.
+      eapply path_NoDup' in Hreach''0;eauto. 
+      destructH. exists x, π0. firstorder;eauto.
+      + eapply subgraph_path';eauto using a_edge_incl.
+      + eapply NoDup_rev in Hreach''3. eapply path_back in Hreach''2.
+        remember (rev π0) as l.
+        destruct l;cbn in *;eauto.
+        specialize (ne_list_nlrcons π0) as Heql'. destructH. subst π0. cbn in *. simpl_nl' Heql.
+        rewrite rev_rcons in Heql. inversion Heql;subst e l.
+        simpl_nl' Hreach''2. subst. inversion Hreach''3;subst. auto.
+  Qed.
+
+  (** about dominance and more about loops **)
+
+  Lemma dom_loop h
+    : forall q: Lab, loop_contains h q -> Dom edge root h q.
+  Proof.
+    intros q Hq. unfold loop_contains,CPath in *. intros π Hπ.
+    destructH. 
+    eapply nin_tl_iff in Hq3;eauto.
+    erewrite path_back in Hq3;eauto.
+    eapply path_app in Hq2; eauto.
+    eapply loop_head_dom in Hq2;eauto. eapply in_nl_conc in Hq2.
+    destruct Hq3;[|subst h;eapply path_front in Hπ; subst q; destruct π;cbn;eauto].
+    destruct Hq2;[contradiction|]. clear - H0. destruct π; cbn in *; eauto.
+  Qed.
+  
+  Lemma dom_dom_acyclic r p q
+    : Dom edge r p q -> Dom a_edge r p q.
+  Proof.
+    intros. unfold Dom in *. intros. apply H. eapply subgraph_path'; eauto using a_edge_incl.
+  Qed.
+
+  Instance loop_contains_Antisymmetric : Antisymmetric Lab eq loop_contains.
+  Proof.
+    unfold Antisymmetric.
+    intros.
+    specialize (a_reachability x) as Hx.
+    specialize (a_reachability y) as Hy.
+    destructH. destructH.
+    eapply dom_loop in H. eapply dom_loop in H0.
+    eapply dom_dom_acyclic in H. eapply dom_dom_acyclic in H0.
+    eapply H in Hy as Hy'. eapply H0 in Hx as Hx'.
+    eapply path_from_elem in Hy;eauto.
+    eapply path_from_elem in Hx;eauto.
+    do 2 destructH.
+    eapply path_path_acyclic';eauto using a_edge_acyclic.
+  Qed.
+
+  Lemma loop_contains_ledge_path
+        (p qh : Lab)
+        (Hledge : p ↪ qh)
+        (q : Lab)
+        (π : ne_list Lab)
+        (Hpath : Path edge q p π)
+        (Hnin : qh ∉ tl (rev π))
+        (x : Lab)
+        (Hin : x ∈ π)
+    : loop_contains qh x.
+  Proof.
+    unfold loop_contains.
+    exists p. specialize (@path_from_elem _ edge _ q p x) as Hx. exploit Hx. destructH.
+    exists ϕ. repeat (split;eauto). contradict Hnin. clear - Hx1 Hnin.
+    induction Hx1; cbn in *;[auto|]. rewrite rev_rcons. cbn. eapply IHHx1 in Hnin.
+    eapply tl_incl;auto.
+  Qed.
+  
+  Lemma loop_contains_trans h h' p
+        (Hloop : loop_contains h h')
+        (Hloop' : loop_contains h' p)
+    : loop_contains h p.
+  Proof.
+    copy Hloop Hloop_save.
+    unfold loop_contains in Hloop,Hloop'.
+    decide (h = h');[subst;eauto|].
+    destructH' Hloop'. destructH' Hloop.
+    exists p1. specialize (@path_app _ edge (h' :<: π) π0 p h' p1) as Hϕ.
+    exploit Hϕ.
+    - econstructor;eauto. eapply minus_subgraph. eauto.
+    - eexists;split;eauto;split;eauto. intro N.
+      specialize (ne_list_nlrcons π) as Hπ. destructH. rewrite Hπ in N. cbn in N. simpl_nl' N.
+      rewrite <-nlconc_to_list in N. unfold rcons in N. rewrite app_assoc in N.
+      rewrite rev_unit in N. cbn in N. eapply in_rev in N.
+      eapply in_app_iff in N. destruct N.
+      + eapply Hloop3. rewrite in_rev in H. clear - H n Hloop2. remember (rev π0) as l.
+        destruct l; eauto. cbn. destruct H;subst;eauto. eapply path_back in Hloop2.
+        specialize (ne_list_nlrcons π0) as Hπ0. destructH. rewrite Hπ0 in Heql.
+        simpl_nl' Heql. rewrite rev_rcons in Heql. inversion Heql;subst. simpl_nl' n. contradiction.
+      + assert (h ∈ π).
+        { rewrite Hπ. simpl_nl. eapply In_rcons. right. auto. }
+        eapply loop_contains_ledge_path in H0;eauto.
+        eapply loop_contains_Antisymmetric in Hloop_save. exploit Hloop_save. contradiction.
+  Qed.
+  
+  Lemma loop_reachs_member (h q : Lab)
+    : loop_contains h q -> h -a>* q.
+  Proof.
+    intros Hloop. cbn.
+    specialize (a_reachability q) as Hπ. destructH.
+    eapply dom_loop in Hloop. eapply dom_dom_acyclic in Hloop.
+    eapply Hloop in Hπ as Hin.
+    eapply path_from_elem in Hπ;eauto. destructH.
+    eexists;eauto.
+  Qed.
+
+  Lemma edge_head_same_loop (* unused *)p h h'
+        (Hedge : edge p h = true)
+        (Hhead : loop_head h)
+        (Hloop : loop_contains h' p)
+    : loop_contains h' h.
+  Proof.
+    eapply no_exit_head in Hhead;[contradiction|].
+  Admitted.
+  
+  Lemma root_loop_root h
+    : loop_contains h root -> h = root.
+  Proof.
+    intros H.
+    eapply dom_loop in H.
+    assert (Path edge root root (ne_single root)) as Hpath;[econstructor|].
+    eapply H in Hpath. destruct Hpath;[subst;auto|contradiction].
+  Qed.
+  
+  Lemma loop_contains_either h1 h2 p
+        (Hloo : loop_contains h1 p)
+        (Hlop : loop_contains h2 p)
+    : loop_contains h1 h2 \/ loop_contains h2 h1.
+  Proof.
+    specialize (a_reachability p) as Hr. destructH.
+    eapply dom_loop in Hloo as Hdom1. eapply dom_dom_acyclic in Hdom1. eapply Hdom1 in Hr as Hr1. 
+    eapply dom_loop in Hlop as Hdom2. eapply dom_dom_acyclic in Hdom2. eapply Hdom2 in Hr as Hr2.
+    eapply path_from_elem in Hr1;eauto.
+    eapply path_from_elem in Hr2;eauto.
+    do 2 destructH.
+    decide (h1 = p);[subst;right;auto|].
+    decide (h2 = p);[subst;left ;auto|].
+    decide (h1 = h2);[subst;left;eauto using loop_contains_self,loop_contains_loop_head|].
+    eapply postfix_order_destruct in Hr4;eauto.
+    destruct Hr4.
+    - left. unfold loop_contains in *. do 2 destructH.
+      exists p1. eapply path_app in Hloo2 as Happ;eauto. exists (π1 :+ tl ϕ).
+      repeat (split;eauto). 2:eauto using subgraph_path',a_edge_incl.
+      enough (h1 ∉ tl ϕ).
+      + contradict Hloo3. eapply tl_incl in Hloo3. eapply in_rev in Hloo3.
+        eapply in_nl_conc in Hloo3. destruct Hloo3;[|contradiction].
+        destr_r π1. simpl_nl. rewrite rev_rcons. cbn. rewrite <-in_rev.
+        simpl_nl' H1. eapply In_rcons in H1. destruct H1;[|auto]. subst a.
+        clear - Hloo2 n.
+        exfalso. contradict n. revert dependent p1.
+        induction l;cbn in *;intros;inversion Hloo2;subst;auto.
+        eapply IHl;eauto.
+      + eapply path_back in Hr2 as Hr2'.
+        eapply path_back in Hr0 as Hr0'.
+        destr_r ϕ0. cbn in Hr2'. simpl_nl' Hr2'. subst a.
+        destr_r ϕ. cbn in Hr0'. simpl_nl' Hr0'. subst a.
+        simpl_nl' H. simpl_nl.
+        eapply acyclic_path_NoDup in Hr2. simpl_nl' Hr2. eapply NoDup_rev in Hr2.
+        inversion H;subst.
+        * eapply rev_rev_eq in H2;repeat rewrite rev_rcons in H2. inversion H2;subst. contradiction.
+        * eapply rev_rev_eq in H0;repeat rewrite rev_rcons in H0. inversion H0;subst.
+          eapply rev_rev_eq in H4. subst l'.
+          intro N. eapply tl_incl in N. eapply postfix_incl in N;[|eauto].
+          rewrite rev_rcons in Hr2. inversion Hr2;subst. eapply in_rev in N; contradiction.
+    - right. unfold loop_contains in *. do 2 destructH.
+      exists p0. eapply path_app in Hlop2 as Happ;eauto. 2: clear Hr0;eauto using subgraph_path',a_edge_incl.
+      exists (π0 :+ tl ϕ0).
+      repeat (split;eauto). 
+      enough (h2 ∉ tl ϕ0).
+      + contradict Hlop3. eapply tl_incl in Hlop3. eapply in_rev in Hlop3.
+        eapply in_nl_conc in Hlop3. destruct Hlop3;[|contradiction].
+        destr_r π0. simpl_nl. rewrite rev_rcons. cbn. rewrite <-in_rev.
+        simpl_nl' H1. eapply In_rcons in H1. destruct H1;[|auto]. subst a.
+        clear - Hlop2 n0.
+        exfalso. contradict n0. revert dependent p0.
+        induction l;cbn in *;intros;inversion Hlop2;subst;auto.
+        eapply IHl;eauto.
+      + eapply path_back in Hr2 as Hr2'.
+        eapply path_back in Hr0 as Hr0'.
+        destr_r ϕ0. cbn in Hr2'. simpl_nl' Hr2'. subst a.
+        destr_r ϕ. cbn in Hr0'. simpl_nl' Hr0'. subst a.
+        simpl_nl' H. simpl_nl.
+        eapply acyclic_path_NoDup in Hr0. simpl_nl' Hr0. eapply NoDup_rev in Hr0.
+        inversion H;subst.
+        * eapply rev_rev_eq in H2;repeat rewrite rev_rcons in H2. inversion H2;subst. contradiction.
+        * eapply rev_rev_eq in H0;repeat rewrite rev_rcons in H0. inversion H0;subst.
+          eapply rev_rev_eq in H4. subst l'.
+          intro N. eapply tl_incl in N. eapply postfix_incl in N;[|eauto].
+          rewrite rev_rcons in Hr0. inversion Hr0;subst. eapply in_rev in N; contradiction.
+  Qed.
+  
+  Lemma dom_path (* unused *)p q
+    : Dom edge root p q -> p -->* q.
+  Proof.
+    intros Hdom.
+    specialize reachability as [π Hπ]. specialize (Hdom π Hπ).
+    eapply path_from_elem in Hπ; eauto using Lab_dec. firstorder.
+  Qed.
+
+  Lemma loop_contains_not_dom (* unused *)h q 
+    : loop_contains h q -> h <> q -> exists p, p ↪ h /\ ~ Dom edge q h p.
+  Proof.
+    intros Hloop Hneq. unfold loop_contains in Hloop. destructH.
+    unfold Dom; eexists; firstorder; eauto.
+    intros H0.
+    eapply nin_tl_iff in Hloop3;eauto. erewrite path_back in Hloop3;eauto.
+    destruct Hloop3;[|subst q;contradiction]. apply H,H0. eauto.
+  Qed.
+  
+  Lemma not_and_iff (A B : Prop) : decidable A -> (~ (A /\ B) <-> ~ A \/ ~ B).
+  Proof.
+    firstorder.
+  Qed.
+
+  Lemma in_tl_in {A : Type} (a : A) (l : list A) : a ∈ tl l -> a ∈ l.
+  Proof.
+    destruct l; cbn in *; eauto.
+  Qed.
+  
+  Lemma dom_loop_contains h p q
+    : loop_contains h q -> ~ loop_contains h p -> Dom edge p h q.
+  Proof.
+    intros Hloop Hnloop.
+    decide (p = q); [subst;contradiction|].
+    unfold loop_contains in Hloop. destructH.
+    eapply nin_tl_iff in Hloop3;eauto; erewrite path_back in Hloop3;eauto.
+    destruct Hloop3 as [Hloop3|Hloop3];[|subst q;eapply dominant_self]. rename π into π1.
+    intros π Hπ.
+(*    assert (p ∈ all_lab) as H0 by (eapply path_in_alllab1;eauto).*)
+    specialize reachability as Hϕ.
+    unfold loop_contains in Hnloop.
+    rewrite DM_not_exists in Hnloop. setoid_rewrite DM_not_exists in Hnloop.
+    eapply path_app in Hloop2;eauto.
+    specialize (Hnloop p0 (π1 :+ tl π)).
+    setoid_rewrite not_and_iff in Hnloop; [setoid_rewrite not_and_iff in Hnloop|].
+    - destruct Hnloop as [Hnloop|Hnloop]; [contradiction|destruct Hnloop].
+      + contradiction.
+      + clear - Hloop3 H.
+        eapply not_not in H.
+        * eapply in_tl_in in H. eapply in_rev in H. eapply in_nl_conc in H. destruct H;[contradiction|].
+          eapply in_tl_in;eauto.
+        * eapply In_dec;eauto.
+    - edestruct path_dec;eauto; firstorder.
+    - edestruct (back_edge_dec p0 h); firstorder.
+      Unshelve. all:eauto. (*TODO: remove *)
+  Qed.
+    Lemma loop_contains_path (* unused *)h q π
+    : CPath h q π -> loop_contains h q -> NoDup π -> forall p, p ∈ π -> loop_contains h p.
+  Proof.
+    intros Hπ Hin Hnd p Hp. 
+    decide (p = h) as [Hph|Hph].
+    - rewrite Hph. eapply loop_contains_self. eapply loop_contains_loop_head; eauto.
+    - destruct (loop_contains_dec h p) as [N|N]; [eauto|exfalso].
+      eapply path_from_elem in Hp; eauto. destructH.
+      eapply dom_loop_contains in N; eauto; cycle 1.
+      eapply postfix_incl in Hp1 as Hp1'; eauto.
+      dependent induction Hp1.
+      + simpl_nl' x. subst ϕ. 
+        eapply Hph. eapply path_back in Hp0; eapply path_back in Hπ. rewrite <-Hp0. eauto.
+      + clear IHHp1. unfold Dom in N.
+        eapply postfix_incl in Hp1. eapply Hp1 in N; eauto.
+        rewrite rcons_nl_rcons in x. eapply ne_to_list_inj in x. rewrite <-x in Hnd.
+        eapply f_equal with (f:=@ne_back Lab) in x. simpl_nl' x. eapply path_back in Hπ. rewrite Hπ in x.
+        subst a.
+        eapply NoDup_nin_rcons; eauto. rewrite rcons_nl_rcons. assumption.
+  Qed.
+
+  Lemma loop_contains_splinter h1 h2 p π
+        (Hloop1 : loop_contains h1 h2)
+        (Hloop2 : loop_contains h2 p)
+        (Hpath : Path edge root p π)
+    : h2 ≻* h1 | π.
+  Proof.
+    eapply dom_loop in Hloop2. eapply Hloop2 in Hpath as Hin.
+    eapply path_to_elem in Hin;eauto. destructH.
+    eapply splinter_prefix;eauto.
+    inversion Hin0;subst h2 a.
+    - eapply dom_loop in Hloop1. eapply Hloop1 in Hin0. rewrite <-H1 in Hin0. inversion Hin0;subst;[|contradiction].
+      econstructor. econstructor. econstructor. econstructor.
+    - cbn in *. econstructor. eapply dom_loop in Hloop1. eapply Hloop1 in Hin0. rewrite <-H3 in Hin0.
+      eapply splinter_single. cbn in *; eauto.
+  Qed.
+
+  (** * preds **)
+
+  Definition preds `{redCFG Lab edge} p : list Lab := filter (decPred_bool (fun q => edge q p)) (elem Lab). 
+
+  Lemma preds_in_same_loop h p q
+        (Hl : loop_contains h p)
+        (Hneq : h <> p)
+        (Hedge : q --> p)
+    : loop_contains h q.
+  Proof.
+    unfold loop_contains in Hl.
+    destructH.
+    eapply path_rcons in Hl2 as Hl2';eauto.
+    exists p0, (π :>: q). repeat (split;eauto).
+    simpl_nl. rewrite rev_rcons. cbn. eapply nin_tl_iff in Hl3;auto.
+    destruct Hl3 as [Hl3|Hl3];[contradict Hl3;eapply in_rev;auto|eapply path_back in Hl2;subst;auto].
+  Qed.
+
+  (** * other facts **)
+
+  Lemma exit_a_edge h p q
+        (Hexit : exit_edge h p q)
+    : a_edge p q = true.
+  Proof.
+    destruct (a_edge p q) eqn:E;[auto|exfalso].
+    eapply no_exit_head;eauto.
+    unfold exit_edge in Hexit. destructH.
+    exists p. unfold back_edge, back_edge_b. unfold_edge_op. split; auto.
+    rewrite negb_true_iff; auto.
+  Qed.
+  
+  Lemma acyclic_path_stays_in_loop (h p q : Lab) π
+        (Hpath : Path a_edge p q π)
+        (Hp : loop_contains h p)
+        (Hq : loop_contains h q)
+    : forall x, x ∈ π -> loop_contains h x.
+  Proof.
+    enough (h ∉ tl (rev π)) as Hnin.
+    - intros.
+      eapply subgraph_path' in Hpath;eauto.
+      eapply (path_from_elem) in Hpath as Hϕ;eauto. destructH.
+      unfold loop_contains in Hq.
+      destructH.
+      exists p0, (π0 :+ tl ϕ); split_conj; auto.
+      + eapply path_app;eauto.
+      + destruct ϕ;cbn;[auto|].
+        assert (e = q) by (clear - Hϕ0; inversion Hϕ0; subst; eauto);subst.
+        rewrite <-nlconc_neconc.
+        rewrite <-neconc_app. rewrite rev_app_distr.
+        replace (tl (rev ϕ ++ rev π0)) with ((tl (rev ϕ)) ++ rev π0).
+        * intro N. eapply in_app_or in N.
+          destruct N.
+          -- apply Hnin. clear - Hϕ1 H0. destruct (ne_list_nlrcons π). destructH. subst. simpl_nl' Hϕ1. simpl_nl.
+             rewrite rev_rcons. cbn.
+             eapply postfix_rev_prefix in Hϕ1. rewrite rev_rcons in Hϕ1.
+             destruct (ne_list_nlrcons ϕ). destructH;subst. simpl_nl' Hϕ1.
+             rewrite nl_cons_lr_shift in Hϕ1. simpl_nl' Hϕ1. rewrite rev_rcons in Hϕ1.
+             simpl_nl' H0. rewrite rev_rcons in H0. cbn in H0.
+             eapply prefix_cons_cons in Hϕ1.
+             eapply prefix_incl in Hϕ1. eapply in_rev in H0. 
+             specialize (Hϕ1 h). eapply Hϕ1.
+             rewrite <-in_rev. right;auto.
+          -- eapply nin_tl_iff in Hq3;auto. destruct Hq3 as [Hq3|Hq3]; [eapply Hq3;eapply in_rev;auto|].
+             eapply path_back in Hq2. rewrite Hq2 in Hq3. subst h.
+             eapply Hnin. clear - Hϕ1.
+             destruct (ne_list_nlrcons π). destructH. rewrite H. simpl_nl. rewrite rev_rcons. cbn.
+             rewrite H in Hϕ1. simpl_nl' Hϕ1.
+             destruct l';[exfalso|];inversion Hϕ1; subst; cbn in *; try congruence'.
+             destruct l'; cbn in *. inversion H2. 1,2: destruct l'; cbn in *; congruence.
+             ++ eapply in_or_app. right;firstorder.
+             ++ eapply postfix_hd_eq in Hϕ1. subst. eapply in_or_app. firstorder.
+        * clear. destruct (ne_list_nlrcons ϕ). destructH. rewrite H. simpl_nl. rewrite rev_rcons. cbn. reflexivity.
+    - intro N.
+      specialize (a_reachability p) as [ϕ Hϕ].
+      eapply dom_loop in Hp.
+      eapply dom_dom_acyclic in Hp.
+      eapply Hp in Hϕ as Hin.
+      eapply path_app in Hpath as Hpath';eauto.
+      eapply acyclic_path_NoDup in Hpath' as Hnd. rewrite <-nlconc_to_list in Hnd.
+      enough (π ++ tl ϕ = rev (tl (rev π)) ++ ϕ).
+      + rewrite H in Hnd.
+        eapply NoDup_app;eauto.
+        rewrite <-in_rev. auto.
+      + clear - Hpath Hϕ.
+        destruct (ne_list_nlrcons π). destructH. subst.
+        simpl_nl. rewrite rev_rcons. cbn. rewrite rev_involutive.
+        eapply path_back in Hpath. simpl_nl' Hpath. subst x.
+        destruct ϕ;cbn in *;simpl_nl.
+        * inversion Hϕ; subst. rewrite app_nil_r. reflexivity.
+        * inversion Hϕ; subst. unfold rcons. rewrite <-app_assoc. cbn. reflexivity.
+  Qed.
+
+  Lemma acyclic_parallel_exit_path h p q π
+        (Hπ : Path a_edge h q π)
+        (Hexit : exit_edge h p q)
+    : forall x, x ∈ tl π -> loop_contains h x.
+  Proof.
+    destruct π;cbn in *;[contradiction|].
+    assert (e = q) by (inversion Hπ;cbn in *;subst;auto);subst.
+    inversion Hπ;subst.
+    intros.
+    eapply acyclic_path_stays_in_loop;eauto.
+    - eapply loop_contains_self;unfold exit_edge in Hexit; destructH ;eauto using loop_contains_loop_head.
+    - eapply exit_pred_loop;eauto.
+      eapply a_edge_incl;eauto.
+  Qed.
+
+  Lemma loop_contains_ledge qh ql
+    : ql ↪ qh -> loop_contains qh ql.
+  Proof.
+    intros. exists ql, (ne_single ql). split_conj;[auto|constructor|cbn]. exact (fun x => x).
+  Qed.
+  
+  Lemma exit_edge_pred_exiting h p q
+        (Hexit : exit_edge h p q)
+        (p' : Lab)
+        (Hedge : edge p' q = true)
+    : exit_edge h p' q.
+  Proof.
+    copy Hexit Hexit'.
+    unfold exit_edge; unfold exit_edge in Hexit. destructH.
+    split_conj;eauto.
+    eapply exit_pred_loop;eauto.
+  Qed.
+  
+  Lemma root_no_acyclic_pred p
+    : a_edge p root <> true.
+  Proof.
+    specialize (a_reachability p) as [π Hπ].
+    intro. eapply a_edge_acyclic;eauto.
+  Qed.
+  
+  Lemma exit_edge_acyclic h qe e
+        (Hexit : exit_edge h qe e)
+    : a_edge qe e = true.
+  Proof.
+    copy Hexit Hexit'.
+    unfold exit_edge in Hexit.
+    destructH.
+    destruct (a_edge qe e) eqn:E;[auto|exfalso].
+    eapply no_exit_head;eauto.
+    eexists; unfold back_edge,back_edge_b; unfold_edge_op.
+    split;eauto. eapply negb_true_iff. auto.
+  Qed.
+
+  Lemma exit_edge_unique_diff_head h qe e
+        (Hexit : exit_edge h qe e)
+        h'
+        (Hloop : loop_contains h' h)
+        (Hnloop : ~ loop_contains h' e)
+    : h' = h.
+  Proof.
+    specialize (a_reachability e) as [π Hπ].
+    inversion Hπ;subst e a.
+    - exfalso. subst π.
+      eapply exit_edge_acyclic in Hexit. exfalso. eapply root_no_acyclic_pred;eauto.
+    - eapply a_edge_incl in H0. eapply exit_pred_loop in H0 as H2;eauto.
+      eapply single_exit with (p:=b) (q:=c).
+      + split;[|split];eauto.
+        eapply loop_contains_trans;eauto.
+      + split;[|split];eauto.
+        contradict Hnloop. eapply loop_contains_trans;eauto.
+  Qed.
+  
+  Lemma exit_edge_in_loop (* unused *) (h1 h2 p1 p2 e1 e2 : Lab)
+        (Hexit : exit_edge h1 p1 e1)
+        (Hexit' : exit_edge h2 p2 e2)
+        (Hloop : loop_contains h1 h2)
+        (Hneq : h1 <> h2)
+    : loop_contains h1 e2.
+    decide (loop_contains h1 e2);[auto|].
+    copy Hexit' Hexit''.
+    unfold exit_edge in Hexit'. destructH.
+    assert (exit_edge h1 p2 e2).
+    {
+      unfold exit_edge. split_conj;cycle 1.
+      + eauto.
+      + eauto.
+      + eauto using loop_contains_trans.
+    }
+    eapply single_exit in Hexit'';eauto. contradiction.
+  Qed.
+
+End cfg.
