cfg/HeadexitsCFG.v
@@ -1,0 +1,374 @@
+Require Export CFGinnermost.
+
+
+(** * head_exits **)
+
+Definition head_exits_edge `{redCFG} h h' q : bool
+  := if decision (exited h' q /\ ~ loop_contains h' h) then true else false. 
+
+Lemma head_exits_edge_spec :
+  forall `{redCFG} h h' q, head_exits_edge h h' q = true -> exists p, exit_edge h' p q.
+Proof.
+  intros. unfold head_exits_edge in H0. decide (exited h' q); cbn;eauto.
+  decide (exited h' q /\ ~ loop_contains h' h);[|congruence]. destructH. contradiction.
+Qed.
+
+Lemma head_exits_edge_spec_iff :
+  forall `{redCFG} h h' q, head_exits_edge h h' q = true <-> (exists p, exit_edge h' p q) /\ ~ loop_contains h' h.
+Proof.
+  intros. unfold head_exits_edge. decide (exited h' q /\ ~ loop_contains h' h).
+  - split;intros;[|reflexivity]. firstorder.
+  - split;intros;[congruence|]. simpl_dec' n. destructH. unfold exited in n.
+    destruct n as [n|n];[simpl_dec' n; specialize (n p)|]; contradiction.
+Qed.
+
+Lemma head_exits_path `{redCFG} h p q :
+  head_exits_edge h p q = true -> exists π, Path a_edge p q π.
+Proof.
+  intros. cbn.
+  eapply head_exits_edge_spec in H0.
+  destructH.
+  copy H0 Hexit.
+  unfold exit_edge in H0. destructH.
+  eapply loop_reachs_member in H1.
+  destructH.
+  exists (q :<: π).
+  eapply exit_a_edge in Hexit.
+  econstructor;eauto.
+Qed.
+
+Lemma head_exits_in_path_head_incl `{redCFG} qh ql π
+      (Hπ : Path (edge ∪ (head_exits_edge qh)) root ql π)
+  : exists ϕ, Path edge root ql ϕ /\ forall (h : Lab), loop_contains h ql -> h ∈ ϕ -> h ∈ π.
+Proof.
+  remember ql as ql'.
+  setoid_rewrite Heqql' at 2.
+  assert (deq_loop ql' ql) as Hdeq by (subst;eapply deq_loop_refl).
+  clear Heqql'.
+  revert dependent ql.
+  induction Hπ;intros;cbn;eauto.
+  - eexists;split;econstructor;eauto. inversion H1;subst;auto. inversion H2.
+  - unfold_edge_op' H0. destruct H0.
+    + specialize (IHHπ b). exploit IHHπ;[eapply deq_loop_refl|]. destructH.
+      exists (c :<: ϕ). split;[econstructor;eauto|].
+      intros. cbn in H2. destruct H2;eauto.
+      eapply Hdeq in H1.
+      decide (h = c);[left;auto|].
+      eapply preds_in_same_loop in H1;eauto.
+    + eapply head_exits_path in H0 as Hψ. destruct Hψ as [ψ Hψ].
+      specialize (IHHπ c). exploit IHHπ.
+      * eapply head_exits_edge_spec in H0. destructH.
+        eapply deq_loop_trans;[eapply deq_loop_exiting;eauto|eapply deq_loop_exited;eauto].
+      * destructH.
+        eexists. split;[eauto using path_app,subgraph_path'|].
+        intros.
+        eapply in_nl_conc in H2. destruct H2.
+        -- left.
+           
+           eapply head_exits_edge_spec in H0. destructH.
+           decide (c = h);[auto|].
+           eapply acyclic_parallel_exit_path in Hψ;eauto.
+           ++ eapply loop_contains_trans in H1;eauto.
+              eapply Hdeq in H1.
+              unfold exit_edge in H0. destructH. contradiction.
+           ++ destruct Hψ;cbn in *;destruct H2. 1-3: contradiction. auto.
+        -- right;eauto using tl_incl. eapply IHHπ1. eapply Hdeq;auto. eapply tl_incl. auto.
+Qed.
+
+Lemma head_exits_back_edge `{redCFG} ql qh h :
+  ((edge ∪ (head_exits_edge h)) ∖ (a_edge ∪ (head_exits_edge h))) ql qh = true <-> ql ↪ qh.
+Proof.
+  unfold back_edge,back_edge_b.
+  unfold_edge_op. split;intros. 
+  - destructH. destruct H1;[eauto|].
+    destruct (head_exits_edge h ql qh);cbn in *;congruence.
+  - split_conj;[firstorder|firstorder|].
+    unfold head_exits_edge.
+    decide (exited ql qh /\ ~ loop_contains ql h);[|cbn;auto].
+    exfalso.
+    unfold exited in a.
+    destructH' a.
+    eapply no_exit_head;eauto.
+    exists ql. unfold back_edge,back_edge_b;conv_bool. unfold_edge_op. eauto.
+Qed.
+
+Lemma head_exits_no_self_loop `{redCFG} h p q : head_exits_edge h p q = true -> p <> q.
+Proof.
+  intros. eapply head_exits_edge_spec in H0.
+  destructH.
+  unfold exit_edge in H0. destructH.
+  eapply loop_contains_loop_head in H1.
+  eapply loop_contains_self in H1.
+  intro N;subst.
+  contradiction.
+Qed.
+
+Lemma head_exits_same_connected `{redCFG} h p q π
+      (Hpath : Path (a_edge ∪ (head_exits_edge h)) p q π)
+  : exists ϕ, Path a_edge p q ϕ.
+Proof.
+  induction Hpath;cbn;eauto.
+  - eexists. econstructor.
+  - destructH. unfold_edge_op' H0. destruct H0.
+    + eexists. econstructor;eauto.
+    + eapply head_exits_path in H0. destructH.
+      eexists; eauto using path_app.
+Qed.
+
+Lemma head_exits_same_connected' (* unused *)`{redCFG} h p q π
+      (Hpath : Path (edge ∪ (head_exits_edge h)) p q π)
+  : exists ϕ, Path edge p q ϕ.
+Proof.
+  induction Hpath;cbn;eauto.
+  - eexists. econstructor.
+  - destructH. unfold_edge_op' H0. destruct H0.
+    + eexists. econstructor;eauto.
+    + eapply head_exits_path in H0. destructH.
+      eapply subgraph_path' in H0;eauto.
+      eexists; eauto using path_app.
+Qed.
+
+
+Lemma head_exits_loop_equivalence `{redCFG} qh h p
+  : loop_contains h p <-> loop_contains' (edge ∪ (head_exits_edge qh)) (a_edge ∪ (head_exits_edge qh)) h p.
+Proof.
+  split;intros.
+  - unfold loop_contains'. unfold loop_contains in H0.
+    destructH.
+    exists p0, π.
+    split_conj.
+    + eapply head_exits_back_edge;eauto.
+    + clear - H0.
+      induction H0;econstructor;eauto. unfold_edge_op. left;auto.
+    + auto.
+  - copy H0 H0'.
+    unfold loop_contains. unfold loop_contains' in H0.
+    destructH.
+    assert (Path (edge ∪ (head_exits_edge qh)) p p0 π -> h ∉ tl (rev π)
+            -> loop_contains h p0
+            -> exists π0, Path edge p p0 π0 /\ h ∉ tl (rev π0)).
+    {
+      clear. intros.
+      induction H0.
+      - exists (ne_single a). split;eauto. econstructor.
+      - exploit' IHPath.
+        + cbn in *. contradict H1.
+          specialize (ne_list_nlrcons π) as Hπ. destructH. subst π.
+          simpl_nl. rewrite rev_rcons. cbn. simpl_nl' H1. rewrite rev_rcons in H1. cbn in *.
+          eapply in_or_app. left;auto.
+        + unfold_edge_op' H3. destruct H3.
+          * exploit IHPath.
+            {
+              eapply preds_in_same_loop;eauto.
+              contradict H1. subst.
+              cbn. ne_r_destruct π. simpl_nl. rewrite rev_rcons. cbn. eapply in_or_app. right;firstorder.
+            }
+            destructH.
+            exists (c :<: π0). split;[econstructor;eauto|].
+            contradict IHPath1.
+            ne_r_destruct π0.
+            simpl_nl. cbn. rewrite rev_rcons. cbn. simpl_nl' IHPath1.
+            rewrite nl_cons_lr_shift in IHPath1. simpl_nl' IHPath1.  rewrite rev_rcons in IHPath1. cbn in *.
+            fold (rcons (rev x0) c) in IHPath1. eapply In_rcons in IHPath1. destruct IHPath1;auto.
+            subst h. exfalso. contradict H1. fold (rcons (rev π) c).
+            ne_r_destruct π.
+            simpl_nl. cbn. rewrite rev_rcons. cbn. eapply in_or_app. right;firstorder.
+          * eapply head_exits_edge_spec in H3 as Hexit. destruct Hexit as [qe Hexit].
+            assert (loop_contains h b) as Hloop.
+            {
+              eapply deq_loop_exiting;eauto.
+              eapply deq_loop_exited;eauto.
+            }
+            exploit IHPath.
+            destructH.
+            eapply head_exits_path in H3. destructH.
+            exists (π1 :+ tl π0).
+            split.
+            -- eapply subgraph_path' in H3; [eapply path_app|];eauto.
+            -- rewrite <-nlconc_to_list.
+               intro N. rewrite rev_app_distr in N.
+               enough (h ∉ rev π1).
+               {
+                 destruct π0;cbn in N;eapply H4;[eapply tl_incl;auto|].
+                 ne_r_destruct π0. cbn in *. simpl_nl' IHPath1. simpl_nl' N. rewrite rev_rcons in N,IHPath1.
+                 cbn in *.
+                 eapply in_app_or in N. destruct N;[exfalso;apply IHPath1|contradiction].
+                 eapply in_or_app. left;auto.
+               }
+               rewrite <-in_rev.
+               clear - H3 Hexit H2 Hloop.
+               decide (h = c).
+               {
+                 subst.
+                 exfalso.
+                 eapply no_exit_head;eauto using loop_contains_loop_head.
+               }      
+               inversion H3;subst.
+               ++ cbn. firstorder.
+               ++ cbn. simpl_dec. split;[auto|].
+                  intro Hin.
+                  eapply acyclic_path_stays_in_loop in Hin;auto;cycle 1.
+                  ** eauto.
+                  ** unfold exit_edge in Hexit. destructH. eapply loop_contains_self.
+                     eapply loop_contains_loop_head;eauto.
+                  ** eapply a_edge_incl in H1.
+                     eapply exit_pred_loop;eauto.
+                  ** eapply loop_contains_Antisymmetric in Hin. exploit Hin. subst.
+                     unfold exit_edge in Hexit; destructH; contradiction.
+    }
+    exists p0.
+    exploit H2.
+    {
+      rewrite head_exits_back_edge in H1. eapply loop_contains_ledge;eauto.
+    }
+    destructH.
+    eexists;split;eauto.
+    eapply head_exits_back_edge;eauto.
+Qed.
+
+
+Lemma head_exits_exit_edge `{redCFG} qh h p q
+      (Hexit : exit_edge' (edge ∪ (head_exits_edge qh)) (a_edge ∪ (head_exits_edge qh)) h p q)
+  : exists p', exit_edge h p' q.
+Proof.
+  unfold exit_edge' in *. destructH.
+  unfold_edge_op' Hexit3.
+  destruct Hexit3.
+  - exists p. unfold exit_edge. split_conj.
+    1,2: rewrite head_exits_loop_equivalence;eauto.
+    auto.
+  - eapply head_exits_edge_spec in H0.
+    destructH. exists p0.
+    unfold exit_edge in *. destructH.
+    split_conj;eauto.
+    + eapply loop_contains_trans;eauto. eapply head_exits_loop_equivalence;eauto.
+    + rewrite head_exits_loop_equivalence;eauto.
+Qed.
+
+Instance head_exits_CFG `(redCFG) qh
+  : redCFG (edge ∪ (head_exits_edge qh)) root (a_edge ∪ (head_exits_edge qh)).
+econstructor;intros.
+{ (* loop_head_dom *)
+  unfold Dom. intros π Hpath.
+  rewrite head_exits_back_edge in H0.
+  eapply loop_contains_ledge in H0.
+  eapply head_exits_in_path_head_incl in Hpath;eauto.
+  destructH.
+  eapply dom_loop in Hpath0 as Hpath';eauto.
+}
+{ (* a_edge_incl *)
+  eapply union_subgraph.
+  - exact a_edge_incl.
+  - firstorder.
+}
+{ (* a_edge_acyclic *)
+  unfold acyclic. intros p q π Hedge Hπ. eapply head_exits_same_connected in Hπ. destructH.
+  unfold union_edge in Hedge; conv_bool. destruct Hedge as [Hedge|Hedge].
+  - eapply a_edge_acyclic; eauto.
+  - eapply head_exits_no_self_loop in Hedge as Hnself.
+    eapply head_exits_path in Hedge. destructH. eapply path_path_acyclic;eauto.
+}
+{ (* reachability *)
+  specialize a_reachability as H0. eapply subgraph_path in H0;eauto.
+  unfold sub_graph,union_edge. firstorder. 
+}
+{ (* single_exit *)
+  fold_lp_cont'.
+  assert (loop_contains h p /\ loop_contains h' p) as [Hloop Hloop'].
+  {
+    unfold exit_edge' in *. do 2 destructH.
+    split; eapply head_exits_loop_equivalence; eauto.
+  }
+  eapply loop_contains_either in Hloop;eauto.
+  destruct Hloop.
+  - eapply head_exits_exit_edge in H0.
+    eapply head_exits_exit_edge in H1.
+    do 2 destructH.
+    eapply single_exit;eauto.
+    unfold exit_edge in *.
+    do 2 destructH.
+    split;auto.
+    eapply loop_contains_trans;eauto.
+  - eapply head_exits_exit_edge in H0.
+    eapply head_exits_exit_edge in H1.
+    do 2 destructH.
+    eapply single_exit;cycle 1; eauto.
+    unfold exit_edge in *.
+    do 2 destructH.
+    split;auto.
+    eapply loop_contains_trans;eauto.
+}
+{ (* no_head_exit *)
+  fold_lp_cont'.
+  intro N. destructH.
+  eapply head_exits_exit_edge in H0. destructH.
+  eapply no_exit_head;eauto.
+  unfold loop_head.
+  exists p0.
+  eapply head_exits_back_edge;eauto.
+}
+{ (* exit_pred_loop *)
+  fold_lp_cont'.
+  eapply head_exits_exit_edge in H0. destructH.
+  unfold_edge_op' H1.
+  destruct H1.
+  - copy H1 Hedge. eapply exit_edge_pred_exiting in H1;eauto.
+    apply (exit_pred_loop (q:=q)) in H1;eauto.
+    rewrite <-head_exits_loop_equivalence;eauto.
+  - eapply head_exits_edge_spec in H1.
+    destructH.
+    copy H0 Hexit.
+    unfold exit_edge in H0.
+    destructH.
+    eapply exit_edge_pred_exiting in H1;eauto.
+    eapply single_exit in Hexit;eauto. subst.
+    rewrite <-head_exits_loop_equivalence. 
+    eauto using loop_contains_self, loop_contains_loop_head.
+}
+{
+  intro Heq.
+  eapply no_self_loops;eauto. subst. unfold_edge_op' H0. destruct H0;[auto|].
+  eapply head_exits_edge_spec in H0. destructH.
+  unfold exit_edge in H0. destructH.
+  exfalso. contradict H0. eauto using loop_contains_loop_head,loop_contains_self.
+}
+{
+  intro N. eapply root_no_pred.
+  unfold_edge_op' N. destruct N.
+  - eauto.
+  - eapply head_exits_edge_spec in H0. destructH. unfold exit_edge in H0.
+    exfalso.
+    destructH.
+    eapply root_no_pred;eauto.
+} 
+Qed.
+
+(* We need LOCAL head exits and also a local headexits property, bc
+ * otherwise every loop head becomes a loop_split of itself and any exit in the imploded graph *)
+Definition head_exits_property `(C : redCFG) qh := forall h p q, exit_edge h p q -> ~ loop_contains h qh
+                                                            -> edge h q = true.
+
+Arguments exit_edge {_ _ _ _} (_).
+
+Lemma head_exits_property_satisfied `(C : redCFG) qh : head_exits_property (head_exits_CFG C qh) qh.
+Proof.
+  unfold head_exits_property. 
+  intros h p q Hexit Hloop. unfold union_edge. conv_bool.
+  eapply head_exits_exit_edge in Hexit.
+  unfold loop_contains in Hloop. unfold back_edge,back_edge_b in Hloop. fold_lp_cont'.
+  rewrite <-head_exits_loop_equivalence in Hloop.
+  right.
+  rewrite head_exits_edge_spec_iff.
+  split;eauto. 
+Qed.
+
+Lemma head_exits_property_a_edge (* unused *)`{C : redCFG} qh 
+  : head_exits_property C qh -> forall h p q : Lab, exit_edge _ h p q -> ~ loop_contains h qh -> a_edge h q = true.
+Proof.
+  intros.
+  eapply H in H0 as H2.
+  - decide (a_edge h q = true);[auto|exfalso].
+    eapply no_exit_head;eauto. unfold loop_head.
+    exists h. unfold back_edge,back_edge_b. unfold_edge_op. split;auto.
+    eapply negb_true_iff,not_true_is_false. auto.
+Qed.
