cfg/ImplodeCFG.v
@@ -1,0 +1,133 @@
+Require Import NePreSuffix CFGgeneral.
+Require Export HeadexitsCFG SubCFG.
+
+Definition implode_nodes `{C : redCFG} (r : Lab)
+  := DecPred (fun p => (deq_loop r p
+                     \/ exists e, exited p e /\ deq_loop r e)).
+
+Lemma implode_nodes_root_inv `{C : redCFG} r
+  : implode_nodes r root.
+Proof.
+  unfold implode_nodes. cbn.
+  left.
+  eapply deq_loop_root.
+Qed.      
+
+Definition purify_implode `{redCFG} h :=
+  purify (implode_nodes_root_inv h) (D:=decide_pred _).
+  
+Definition impl_list `{redCFG} (h : Lab) :=
+  filter (DecPred (fun q : Lab => (loop_contains h q \/ exited h q)
+                        /\ (deq_loop h q
+                            \/ exists e, exited q e
+                                   /\ deq_loop h e
+                           )
+                  )
+         ).
+
+
+Lemma implode_nodes_back_edge (* unused *)`{redCFG} h p q
+      (Hhead : back_edge' (restrict_edge' edge (implode_nodes h)) (restrict_edge' a_edge (implode_nodes h)) p q)
+  : p ↪ q.
+Proof.
+  unfold back_edge' in *.
+  unfold_edge_op' Hhead. destructH.
+  decide (implode_nodes h p);[|contradiction].
+  decide (implode_nodes h q);[|contradiction].
+  destruct Hhead1 as [Hhead1|[Hhead1|Hhead1]];cbn in *.
+  2,3:congruence.
+  unfold back_edge,back_edge_b. unfold_edge_op. split;auto.
+Qed.
+
+Instance implode_CFG `(H : redCFG) h7 (Hhe : head_exits_property H h7)
+  : @redCFG (finType_sub_decPred (implode_nodes h7))
+            (restrict_edge edge (implode_nodes h7))
+            (↓ purify_implode h7)
+            (restrict_edge a_edge (implode_nodes h7)).
+Proof.
+  eapply sub_CFG;intros.
+  - specialize (a_reachability p) as [π Hπ].
+    revert dependent p. revert dependent π.
+    specialize (well_founded_ind (R:=(@StrictPrefix' Lab)) (@StrictPrefix_well_founded Lab)
+                                 (fun π : ne_list Lab => forall (p : Lab),
+                                      implode_nodes h7 p ->
+                                      Path a_edge root p π
+                                      -> exists π0, Path (restrict_edge' a_edge (implode_nodes h7)) root p π0))
+      as WFind.
+    eapply WFind.
+    intros ? IHwf ? ? ?. clear WFind.
+    destruct H1.
+    + eexists; econstructor.
+    + unfold implode_nodes in H0. cbn in H0.
+      decide (implode_nodes h7 b).
+      * specialize (IHwf π). exploit IHwf;[econstructor;econstructor|].
+        destructH.
+        eexists; econstructor;eauto.
+        unfold_edge_op. split_conj;auto.
+      * unfold implode_nodes in n. cbn in n. simpl_dec' n.
+        destructH.
+        simpl_dec' n1. simpl_dec' n1.  
+        enough (exists h, exit_edge _ h b c).
+        {
+          destructH.
+          enough (h ∈ π).
+          {
+            eapply path_to_elem in H4;eauto. destructH.
+            specialize (IHwf ϕ).
+            assert (implode_nodes h7 h) as Himpl.
+            {
+              destruct H0.
+              * right. exists c. split;[exists b|];eauto.
+              * exfalso.
+                destructH. eapply no_exit_head;eauto.
+                unfold exited,exit_edge in H4; destructH. eauto using loop_contains_loop_head.
+            }
+            exploit IHwf.
+            - eapply prefix_ex_cons in H6. destructH. econstructor. cbn. eauto.
+            - destructH. 
+              exists (c :<: π0). econstructor;eauto. unfold_edge_op. split_conj;eauto.
+              eapply head_exits_property_a_edge;eauto.
+              contradict n0.
+              eapply loop_contains_deq_loop in n0.
+              eapply eq_loop_exiting in H3.
+              eapply eq_loop2;eauto.
+          }
+          eapply dom_loop;[unfold exit_edge in H3;destructH;eauto|].
+          eapply subgraph_path';eauto.
+        }
+        simpl_dec' n0. simpl_dec' n0.
+        destructH.
+        exists x. unfold exit_edge;split_conj;eauto using a_edge_incl.
+        destruct H0.
+        -- contradict n3. eauto.
+        -- destructH.
+           destruct H3 as [q Hexit]. 
+           decide (x = c).
+           ++ exfalso. subst. eapply loop_reachs_member in n2. destructH.
+              eapply a_edge_acyclic;eauto.
+           ++ 
+              intro N.
+              eapply exit_edge_unique_diff_head in Hexit;auto;cycle 1.
+              ** exact N.
+              ** contradict n3. eapply H4;eauto.
+              ** contradiction.
+  - rewrite loop_contains'_basic in H1.
+    unfold loop_contains in H1. rename H1 into Hloop.
+    destructH.
+    exists p0.
+    revert dependent p.
+    induction π;intros;inversion Hloop2;subst.
+    + exists (ne_single a). split_conj;eauto.
+      * unfold_edge_op. split_conj;eauto using back_edge_incl.
+        -- admit. (*left;eapply deq_loop_refl.*)
+        -- left. unfold back_edge,back_edge_b in Hloop0. unfold_edge_op' Hloop0. firstorder.
+      * econstructor.
+    + admit. (* FIXME: give intuition *)
+Admitted.
+
+Lemma implode_CFG_elem `{C : redCFG} (p h : Lab) (Himpl : implode_nodes h p)
+  : finType_sub_decPred (implode_nodes h).
+Proof.
+  econstructor. unfold pure. instantiate (1:=p).
+  decide (implode_nodes h p);eauto.
+Defined.
