cfg/OptLoopCFG.v
@@ -1,0 +1,72 @@
+Require Export LoopCFG.
+
+Instance opt_loop_CFG' `(C : redCFG) (h : Lab)
+  : let d := (@decision (@loop_head _ _ _ _ C h) (loop_head_dec _)) in
+    let Lab' := @finType_sub_decPred Lab (@loop_nodes Lab edge root a_edge C h) in
+    @redCFG (if d then Lab' else Lab)
+            ((if d
+                 return ((if d then Lab' else Lab)
+                         -> (if d then Lab' else Lab) -> bool) then
+                (@restrict_edge Lab edge (@loop_nodes Lab edge root a_edge C h))
+              else
+                edge))
+            (match d
+                   return (eqtype (type (if d then Lab' else Lab))) with
+             | left H => (↓ purify_head H)
+
+                 (*@finType_sub_elem Lab h (@loop_nodes Lab edge root a_edge C h)
+                                           (or_introl (@loop_contains_self Lab edge root a_edge C h H)))*)
+             | right _ => root
+             end)
+            ((if d as d
+                 return ((if d then Lab' else Lab)
+                         -> (if d then Lab' else Lab) -> bool) then
+                (@restrict_edge Lab a_edge (@loop_nodes Lab edge root a_edge C h))
+              else
+                a_edge)).
+Proof.
+  intros.
+  destruct d; eauto. 
+Defined.
+
+Definition opt_loop_CFG_type `(C : redCFG) (d : option {h : Lab | loop_head h})
+  := (match d with
+      | Some (exist _ h H) => loop_CFG_type H
+      | None => Lab
+      end). 
+
+Instance opt_loop_CFG `(C : redCFG) (d : option {h : Lab | loop_head h})
+  : @redCFG (opt_loop_CFG_type d)
+            (match d
+                   return ((opt_loop_CFG_type d) -> (opt_loop_CFG_type d) -> bool) with
+             | Some (exist _ h H) => (@restrict_edge Lab edge (@loop_nodes Lab edge root a_edge C h))
+             | None => edge
+             end)
+            (match d
+                   return (eqtype (type (opt_loop_CFG_type d))) with
+             | Some (exist _ h H) => (↓ purify_head H) 
+             | None => root
+             end)
+            (match d
+                   return ((opt_loop_CFG_type d) -> (opt_loop_CFG_type d) -> bool) with
+             | Some (exist _ h H) => (@restrict_edge Lab a_edge (@loop_nodes Lab edge root a_edge C h))
+             | None => a_edge
+             end).
+Proof.
+  intros.
+  destruct d; [destruct s|]; eauto.
+Defined.
+
+Lemma opt_loop_CFG_elem (* unused *)`{C : redCFG} (p : Lab)
+      (d : option {h : Lab | loop_head h})
+      (Hd : match d with
+            | Some (exist _ h _) => loop_contains h p
+            | None => True
+            end)
+  : opt_loop_CFG_type d.
+Proof.
+  destruct d;[|exact p].
+  destruct s. eapply loop_CFG_elem; eauto.
+Defined.
+
+Arguments opt_loop_CFG {_ _ _ _} _.
