cfg/SubCFG.v
@@ -1,0 +1,444 @@
+Require Export CFGloop CFGTac.
+
+Section Restr.
+  Context `{C : redCFG}.
+  
+  Notation "p '-a>b' q" := (a_edge p q) (at level 55).
+  Notation "p '-a>' q" := (p -a>b q = true) (at level 55).
+  Notation "p '-->b' q" := (edge p q) (at level 55).
+  Notation "p '-->' q" := (p -->b q = true) (at level 55, right associativity).
+  
+  Definition finType_sub_elem (* unused *)(h : Lab) (p : decPred Lab) (H : p h)
+    := (exist (fun x : Lab => pure p x) h (purify H)).
+
+  
+  Lemma restrict_edge_intersection (A : finType) (f : A -> A -> bool) (p : decPred A) x y
+    : restrict_edge f (p:=p) x y = restrict_edge' f p (`x) (`y).
+  Proof.
+    clear Lab edge root a_edge C.
+    destruct x,y. 
+    unfold restrict_edge',restrict_edge,intersection_edge. cbn.
+    symmetry. destruct (f x x0);cbn;conv_bool;[split;eapply (pure_equiv (D:=decide_pred p));auto|reflexivity].
+  Qed.
+End Restr.
+
+Notation "↓ H" := (exist (fun x => pure (@predicate (eqtype (type _)) _) x) _ H) (at level 70).
+
+Arguments restrict_edge {_}.
+
+(** * sub_CFG **)
+
+Open Scope prg.
+
+Lemma original_path (L : Type) (P : decPred L) f π (r p : @subtype _ P (decide_pred P))
+      (Hpath : Path (fun x y : subtype P => f (`x) (`y)) r p π)
+  : Path f (`r) (`p) (ne_map (@proj1_sig L _) π).
+Proof.
+  induction Hpath.
+  - cbn. econstructor.
+  - cbn. econstructor;eauto.
+Qed.
+
+Lemma original_path' (L : finType) (P : decPred L) f π (r p : @subtype _ P (decide_pred P))
+      (Hpath : Path (fun x y : subtype P (D:=decide_pred P) => f (`x) (`y)) r p π)
+  : Path (restrict_edge' f P) (`r) (`p) (ne_map (@proj1_sig L _) π).
+Proof.
+  induction Hpath.
+  - cbn. econstructor.
+  - cbn. econstructor;eauto.
+    rewrite <-restrict_edge_intersection.
+    unfold restrict_edge. auto.
+Qed.
+
+Definition list_to_ne (* unused *)(A : Type) (l : list A) : option (ne_list A)
+  := match l with
+     | [] => None
+     | a :: l => Some (a :< l)
+     end.     
+
+Lemma toSubList_eq (A : Type) (l : list A) (P : decPred A)
+      (Hl : forall a, a ∈ l -> P a)
+  : map (proj1_sig (P:=fun x => pure P x (D:=decide_pred P))) (toSubList l P) = l.
+  induction l; cbn; eauto.
+  decide (P a);cbn.
+  - f_equal. eapply IHl. intros;eauto.
+  - exfalso; eapply n; eauto.
+Qed.
+
+Lemma restrict_path_sat_P (L : finType) p q π (f : L -> L -> bool) (P : decPred L)
+      (Hp : P p)
+      (Hπ : Path (restrict_edge' f P) p q π)
+      (x : L)
+      (Hin : x ∈ π)
+  : P x.
+Proof.
+  induction Hπ.
+  - destruct Hin;[subst;auto|cbn in *;contradiction].
+  - cbn in Hin. destruct Hin;[subst|eauto].
+    unfold restrict_edge',intersection_edge in H. conv_bool. firstorder.
+Qed.
+
+Ltac cstr_subtype H :=
+  let Heqqh := fresh "H" in 
+  lazymatch type of H with
+  | @predicate (eqtype (type ?Lab)) ?P ?y
+    => assert (` (exist (fun x => pure P x (D:=decide_pred P)) y (purify H)) = y) as Heqqh by (cbn;auto);
+      rewrite <-Heqqh in *; clear Heqqh
+  end.
+
+Ltac collapse x y :=
+        let Q := fresh "Q" in 
+        assert (purify x (D:=decide_pred _) = purify y (D:=decide_pred _)) as Q by (eapply pure_eq);
+        rewrite Q in *;
+        clear Q.
+  
+Ltac push_purify H :=
+  let H' := fresh "H" in 
+  eapply pure_equiv in H as H';
+  assert (H = purify H') by eapply pure_eq;
+  subst H.
+
+Lemma original_path_reverse:
+  forall (L : finType) (r : L) (π : ne_list L) (f : L -> L -> bool) (P : decPred L) (Hr : P r) (x : L) (Hx : P x) l,
+    Path (restrict_edge' f P) r (` (↓ purify Hx (D:=decide_pred P)))
+         (ne_map (proj1_sig (P:=fun x0 : L => pure P x0)) l) ->
+    forall p : P x, Path (restrict_edge f P) (↓ purify Hr) (↓ purify Hx) l.
+Proof. 
+  intros L r π f P Hr x Hx l Hπ p.
+  cbn in *.
+  revert dependent x.
+  induction l;intros;cbn.
+  - destruct a.
+    cbn in *. assert (x0 = x /\ r = x) as [Q1 Q2] by (split; inversion Hπ;subst;auto);subst.
+    push_purify p0.
+    collapse Hr Hx. collapse Hx H.
+    econstructor.
+  - destruct a.
+    cbn in *. assert (x0 = x) as Q by (inversion Hπ;subst;auto);subst.
+    push_purify p0.
+    collapse Hx H.
+    inversion Hπ;subst.
+    assert (P b) as Hb.
+    { unfold restrict_edge',minus_edge,intersection_edge in H4; conv_bool. firstorder. }
+    cstr_subtype Hb.
+    econstructor.
+    + eapply IHl;eauto. 
+    + rewrite restrict_edge_intersection. cbn in *; eauto.
+      Unshelve. cbn. auto.
+Qed.
+
+Lemma restrict_edge_path_equiv (L : finType) r x π (f : L -> L -> bool) (P : decPred L)
+      (Hr : P r)
+      (Hx : P x)
+      (Hπ : Path (restrict_edge' f P) r x π)
+  : match toSubList π P with
+    | a :: l => Path (restrict_edge f P) (↓ (purify Hr)) (↓ (purify Hx)) (a :< l)
+    | nil => False
+    end.
+Proof.
+  revert dependent x.
+  induction π;intros.
+  - cbn.
+    assert (a = x /\ r = x) as [Q1 Q2] by (split;inversion Hπ;auto);subst.
+    decide (P x).
+    + cbn.
+      collapse Hr Hx. collapse Hx p. econstructor.
+    + contradiction. 
+  - assert (a = x);subst.
+    { inversion Hπ. reflexivity. }
+    rewrite nlcons_necons in Hπ.
+    specialize (restrict_path_sat_P Hr Hπ) as Hin.
+    cstr_subtype Hx.
+    setoid_rewrite <-toSubList_eq with (P:=P) in Hπ.
+    2: { cbn in Hin. intros; eapply Hin. simpl_nl. cbn. firstorder. }
+    rewrite <-ne_map_nlcons in Hπ.
+    cbn.
+    decide (P x).
+    + 
+      collapse Hx p.
+      eapply original_path_reverse;eauto.
+    + contradiction.
+Qed.
+
+Lemma subtype_ne_map (A : Type) (P : decPred A) (x : @subtype _ P (decide_pred P))
+      (l : ne_list (@subtype _ P (decide_pred P)))
+      (Hin : (` x) ∈ ne_map (proj1_sig (P:=fun x => pure P x)) l)
+  : x ∈ l.
+Proof.
+  induction l.
+  - cbn in *. destruct Hin;[left;eapply subtype_extensionality;auto|contradiction].
+  - cbn in *. destruct Hin;[left;eapply subtype_extensionality;auto|].
+    auto.
+Qed.
+
+Lemma restrict_edge_subgraph (A : finType) (f g : A -> A -> bool) P
+      (Hsub : sub_graph f g)
+  : sub_graph (restrict_edge f P) (restrict_edge g P).
+Proof.
+  unfold sub_graph in *. intros. unfold restrict_edge in *. eapply Hsub; auto.
+Qed.
+
+Lemma dom_restrict_subtype `{redCFG} r qh ql P 
+      (Hdom : Dom (restrict_edge' edge P) r qh ql)
+      (Hr : P r)
+      (Hh : P qh)
+      (Hl : P ql)
+  : Dom (restrict_edge edge P) (↓ (purify Hr)) (↓ (purify Hh)) (↓ (purify Hl)).
+Proof.
+  unfold Dom. intros.
+  eapply original_path' in H0. cbn in *.
+  unfold Dom in Hdom.
+  eapply Hdom in H0 as H0'.
+  (*  eapply loop_head_dom with (qh0:=qh) in H0 as H0'.*)
+  - cstr_subtype  Hh.
+    eapply subtype_ne_map in H0';auto.
+Qed.
+
+Lemma restrict_back_edge_intersection (L : finType) (edge a_edge : L -> L -> bool) (P : decPred L)
+      (x y : finType_sub P (decide_pred P))
+  : (restrict_edge edge P ∖ restrict_edge a_edge P) x y
+    = (restrict_edge' edge P ∖ restrict_edge' a_edge P) (` x) (` y).
+Proof.
+  destruct x,y.
+  unfold_edge_op. unfold restrict_edge. cbn. 
+  symmetry. destruct (edge x x0),(a_edge x x0);cbn;conv_bool.
+  3,4: reflexivity.
+  2: split;[split;eapply (pure_equiv (D:=decide_pred P));eauto|reflexivity].
+  right.
+  decide (P x); decide (P x0); cbn; auto; eapply pure_equiv in p; eapply pure_equiv in p0;
+    try contradiction; split; auto.
+Qed.           
+
+Lemma restrict_back_edge (L : finType) (edge a_edge : L -> L -> bool) (p h : L) (P : decPred L)
+      (Hp : P p)
+      (Hh : P h)
+      (Hback : (restrict_edge edge P ∖ restrict_edge a_edge P) (↓ (purify Hp)) (↓ (purify Hh)) = true)
+  : (edge ∖ a_edge) p h = true.
+Proof.
+  unfold minus_edge,intersection_edge in *; conv_bool.
+  destructH.
+  split.
+  - rewrite restrict_edge_intersection in Hback0. cbn in *. unfold restrict_edge',intersection_edge in Hback0.
+    conv_bool. firstorder.
+  - rewrite negb_true_iff in Hback1. eapply negb_true_iff.
+    rewrite restrict_edge_intersection in Hback1. cbn in *. unfold restrict_edge',intersection_edge in Hback1.
+    conv_bool. firstorder.
+Qed.
+
+Lemma map_tl (A B : Type) (f : A -> B) (l : list A)
+  : map f (tl l) = tl (map f l).
+Proof.
+  induction l; cbn in *; eauto.
+Qed.
+
+Lemma restrict_loop_contains:
+  forall (Lab : finType) (edge : Lab -> Lab -> bool) (a_edge : Lab -> Lab -> bool)
+    (P : decPred Lab) (h : Lab) (Hh : pure P h) (p : Lab) 
+    (Hp : pure P p),
+    loop_contains' (restrict_edge edge P) (restrict_edge a_edge P) (↓ Hh) (↓ Hp) -> loop_contains' edge a_edge h p.
+Proof.
+  intros Lab edge a_edge P h Hh p Hp HloopA.
+  unfold loop_contains' in *.
+  destructH. cbn in *.
+  eapply original_path in HloopA2. destruct p0. cbn in *.
+  push_purify Hh.
+  push_purify p0.
+  eapply restrict_back_edge in HloopA0.
+  exists x;eexists; split_conj; eauto.
+  contradict HloopA3. cstr_subtype H. cbn in *.
+  rewrite <-to_list_ne_map in HloopA3.
+  rewrite <-map_rev in HloopA3.
+  rewrite <-map_tl in HloopA3.
+  rewrite in_map_iff in HloopA3.
+  destructH. destruct x0. cbn in *.
+  subst.
+  replace (purify H) with p0;auto.
+  eapply pure_eq.
+Qed.
+
+Lemma toSubList_rcons (A : Type) (l : list A) (P : decPred A) (a : A)
+  : toSubList (l ++ [a]) P (D:=decide_pred P) = toSubList l P ++ match decision (P a) with
+                                                                 | left Ha => [exist (pure P) a (purify Ha)]
+                                                                 | right _ => nil
+                                                                 end.
+Proof.
+  induction l; cbn; eauto.
+  - decide (P a); decide (P a); [cbn;eauto;f_equal;f_equal;eapply pure_eq|contradiction|contradiction|reflexivity].
+  - decide (P a0);decide (P a0). 2,3: contradiction. 
+    + cbn. f_equal. eapply IHl. 
+    + eapply IHl.
+Qed.
+
+Lemma toSubList_rev (A : Type) (l : list A) (P : decPred A)
+  : toSubList (rev l) P (D:=decide_pred P) = rev (toSubList l P).
+Proof.
+  induction l; cbn in *; eauto.
+  rewrite toSubList_rcons.
+  decide (P a);decide (P a); try contradiction.
+  - cbn. rewrite IHl.
+    f_equal. f_equal. f_equal. apply pure_eq.
+  - rewrite app_nil_r. eauto.
+Qed.
+
+Lemma toSubList_tl_incl (A : Type) (l : list A) (P : decPred A)
+  : tl (toSubList l P) ⊆ toSubList (tl l) P (D:=decide_pred P).
+Proof.
+  induction l; cbn in *; eauto.
+  decide (P a);cbn.
+  - reflexivity.
+  - eapply tl_incl.
+Qed.  
+
+Lemma loop_contains_restrict' `{redCFG} h q (P : decPred Lab)
+      (Hh : P h)
+      (Hq : P q)
+      (Hloop : loop_contains' (restrict_edge' edge P) (restrict_edge' a_edge P) h q)
+  : loop_contains' (restrict_edge edge P) (restrict_edge a_edge P) (↓ (purify Hh)) (↓ (purify Hq)).
+Proof.
+  unfold loop_contains' in *.
+  destructH.
+  decide (P p).
+  - eapply restrict_edge_path_equiv in Hloop2 as Hloop2'.
+    destruct (toSubList π P) eqn:E;
+      [contradiction|].
+    exists (↓ (purify p0)), (s :< l).
+    split_conj.
+    + unfold minus_edge in *. conv_bool. destruct Hloop0. split_conj; rewrite restrict_edge_intersection;cbn;eauto.
+    + eapply Hloop2'.
+    + Set Printing Coercions. simpl_nl. setoid_rewrite <-E. Unset Printing Coercions.
+      contradict Hloop3. rewrite <-toSubList_eq with (P:=P);[|intros;eapply restrict_path_sat_P with (p:=q);eauto].
+      2: { apply in_rev. apply tl_incl. auto. }
+      eapply in_map_iff. exists (↓ purify Hh). split;cbn;auto.
+      eapply toSubList_tl_incl. rewrite toSubList_rev. auto.
+  - exfalso.
+    unfold restrict_edge', minus_edge, intersection_edge in Hloop0. conv_bool. destructH.
+    contradiction.
+Qed.
+
+Lemma restrict_exit_edge `{C : redCFG} (P : decPred Lab)
+      (p : Lab)
+      (Hp : P p)
+      (q : Lab)
+      (Hq : P q)
+      (h : Lab)
+      (Hh : P h)
+      (Hloop : forall h p : Lab, (exists x, (restrict_edge' edge P ∖ restrict_edge' a_edge P) x h = true)
+                            -> loop_contains' edge a_edge h p
+                            -> P p
+                            -> loop_contains' (restrict_edge' edge P) (restrict_edge' a_edge P) h p)
+      (HloopB : loop_contains' (restrict_edge edge P) (restrict_edge a_edge P) (↓ (purify Hh)) (↓ (purify Hp)))
+      (HnloopB : ~ loop_contains' (restrict_edge edge P) (restrict_edge a_edge P) (↓ (purify Hh)) (↓ (purify Hq)))
+      (HedgeB : restrict_edge' edge P (` (↓ (purify Hp))) (` (↓ (purify Hq))) = true)
+  : exit_edge h p q.
+Proof.
+  unfold exit_edge; split_conj.
+  - eapply restrict_loop_contains;eauto.
+  - contradict HnloopB. eapply loop_contains_restrict'; eauto.
+    eapply Hloop;eauto. unfold loop_contains' in HloopB. destructH.
+    clear - HloopB0.
+    destruct p0. push_purify p.
+    exists x.
+    unfold minus_edge,intersection_edge in *. conv_bool. repeat rewrite restrict_edge_intersection in HloopB0.
+    cbn in *. firstorder.
+  - eapply intersection_subgraph1; unfold restrict_edge' in HedgeB;eauto.
+Qed.
+
+Instance sub_CFG
+        `{C : redCFG}
+        (P : decPred Lab)
+        (HP : P root)
+        (Hreach : forall p, P p -> exists π, Path (restrict_edge' a_edge P) root p π)
+        (Hloop : forall h p, (exists x, (restrict_edge' edge P ∖ restrict_edge' a_edge P) x h = true)
+                        -> loop_contains' edge a_edge h p
+                        -> P p
+                        -> loop_contains' (restrict_edge' edge P) (restrict_edge' a_edge P) h p)
+  : @redCFG (finType_sub_decPred P)
+            (restrict_edge edge P)
+            (↓ (purify HP))
+            (restrict_edge a_edge P).
+econstructor.
+{ (* loop_head_dom *)
+  intros.
+  destruct qh as [qh Qh].
+  destruct ql as [ql Ql].
+  push_purify Qh.
+  push_purify Ql.
+  eapply dom_restrict_subtype.
+  unfold Dom.
+  intros π Hπ.
+  eapply loop_head_dom.
+  - eapply restrict_back_edge in H. unfold back_edge, back_edge_b;eauto.
+  - eapply subgraph_path' in Hπ;eauto. eapply intersection_subgraph1.
+}
+{ (* a_edge_incl *)
+  eapply restrict_edge_subgraph;eauto.
+}
+{ (* a_edge_acyclic *)
+  unfold acyclic. intros.
+  rewrite restrict_edge_intersection in H. destruct p, q; cbn in *.
+  eapply a_edge_acyclic.
+  - eapply intersection_subgraph1;eauto.
+  - eapply original_path in H0;eauto.
+}
+{ (* a_reachability *)
+  destruct q.
+  exploit Hreach; [eapply (pure_equiv (D:=decide_pred P));auto|].
+  destructH.
+  push_purify p.
+  eapply restrict_edge_path_equiv in Hreach.
+  destruct (toSubList π P);[contradiction|]. eauto.
+}
+{ (* single_exit *)
+  intros h p q [HloopA [HnloopA HedgeA]] h' [HloopB [HnloopB HedgeB]].
+  rewrite restrict_edge_intersection in HedgeA,HedgeB.
+  destruct p as [p Hp]. destruct q as [q Hq].
+  destruct h as [h Hh]. destruct h' as [h' Hh'].
+  eapply subtype_extensionality. cbn. 
+  apply (@single_exit _ _ _ _ C h p q).
+  all: push_purify Hh; push_purify Hh'; push_purify Hq; push_purify Hp.
+  all: fold_lp_cont'; eapply restrict_exit_edge; eauto.
+}
+{ (* no_exit_head *)
+  intros h p q [HloopA [HnloopA HedgeA]] Hhead.
+  fold_lp_cont'.
+  destruct h,p,q.
+  eapply no_exit_head.
+  - push_purify p0; push_purify p; push_purify p1. eapply restrict_exit_edge;eauto.
+    rewrite restrict_edge_intersection in HedgeA. eauto.
+  - destruct Hhead. destruct x2. exists x2. eapply restrict_back_edge;eauto.
+    Unshelve.
+    exact P.
+    apply pure_equiv with (D:=decide_pred P);eauto.
+    apply pure_equiv with (D:=decide_pred P);eauto.
+}
+{ (* exit_pred_loop *)
+  intros ? ? ? ? [HloopA [HnloopA HedgeA]] Hedge1.
+  destruct h,q,qe,e.
+  fold_lp_cont'. 
+  push_purify p0. push_purify p1. push_purify p2. push_purify p.
+  eapply loop_contains_restrict'.
+  eapply Hloop.
+  - clear - HloopA. destruct HloopA as [x3 [_ [Hthis _]]].
+    destruct x3. push_purify p.
+    exists x0. cstr_subtype H. cstr_subtype H2. rewrite <-restrict_back_edge_intersection. eauto.
+  - eapply exit_pred_loop with (h:=x).
+    eapply (restrict_exit_edge (p:=x1) (Hp:=H0) (q:=x2)(Hq:=H1)(Hh:=H2));eauto.
+    + rewrite restrict_edge_intersection in HedgeA;eauto.
+    + rewrite restrict_edge_intersection in Hedge1.
+      eapply intersection_subgraph1;eauto.
+  - auto.
+}
+{ (* no_self_loops *)
+  intros.
+  destruct q. destruct p.
+  intro Heq. eapply subtype_extensionality in Heq.
+  eapply no_self_loops;eauto.
+}
+{ (* root_no_pred *)
+  intros.
+  destruct p. push_purify p. intro N.
+  eapply root_no_pred.
+  rewrite restrict_edge_intersection in N.
+  eapply intersection_subgraph1 in N. cbn in N. eauto.
+}
+Qed.
